DynamoDbEncryption/dafny/DynamoDbEncryption/test/BeaconTestFixtures.dfy
@@ -12,11 +12,14 @@ module BeaconTestFixtures {
   import DDB = ComAmazonawsDynamodbTypes
   import SE = AwsCryptographyStructuredEncryptionTypes
   import KeyStore
+  import Seq
   import KMS = Com.Amazonaws.Kms
   import DDBC = Com.Amazonaws.Dynamodb
   import KTypes = AwsCryptographyKeyStoreTypes
   import SI = SearchableEncryptionInfo
   import Aws.Cryptography.Primitives
+  import MaterialProviders
+  import MPT = AwsCryptographyMaterialProvidersTypes
 
   method expect_equal<T(==)>(a: T, b: T)
     ensures a == b
@@ -176,11 +179,17 @@ module BeaconTestFixtures {
     ensures output.ValidState()
     ensures version.keyStore == output.store
     ensures fresh(output.client.Modifies)
-    ensures fresh(output.cache)
   {
-    var cache := new SI.DumbCache();
     var client :- expect Primitives.AtomicPrimitives();
-    return SI.KeySource(client, cache, version.keyStore, SI.LiteralKey([1,2,3,4,5]));
+    var keyNames := Seq.Map((b : StandardBeacon) => b.name, version.standardBeacons);
+    var keys :- expect SI.GetHmacKeys(client, keyNames, key);
+    var mpl :- expect MaterialProviders.MaterialProviders();
+    var input := MPT.CreateCryptographicMaterialsCacheInput(
+      entryCapacity := 3,
+      entryPruningTailSize := None
+    );
+    var cache :- expect mpl.CreateCryptographicMaterialsCache(input);
+    return SI.KeySource(client, version.keyStore, SI.LiteralLoc(keys), cache, 0);
   }
 
   const SimpleItem : DDB.AttributeMap := map[
