DynamoDbEncryption/dafny/DynamoDbEncryptionTransforms/src/TransactWriteItemsTransform.dfy
@@ -90,7 +90,7 @@ module TransactWriteItemsTransform {
 
         //= specification/dynamodb-encryption-client/ddb-sdk-integration.md#encrypt-before-transactwriteitems
         //# - Beacons MUST be [added](ddb-support.md#addbeacons).
-        var beaconItem :- AddBeacons(tableConfig, item.Put.value.Item);
+        var beaconItem :- AddSignedBeacons(tableConfig, item.Put.value.Item);
 
         //= specification/dynamodb-encryption-client/ddb-sdk-integration.md#encrypt-before-transactwriteitems
         //# - If the request is validated,
@@ -102,13 +102,15 @@ module TransactWriteItemsTransform {
           EncTypes.EncryptItemInput(plaintextItem:=beaconItem)
         );
         var encrypted :- MapError(encryptRes);
+        // TODO - extract KeyId from encryption output if Multi
+        var beaconAttrs :- GetEncryptedBeacons(tableConfig, item.Put.value.Item, None);
 
         //= specification/dynamodb-encryption-client/ddb-sdk-integration.md#encrypt-before-transactwriteitems
         //# - The PutItem request's `Item` field MUST be replaced
         //# with a value that is equivalent to
         //# the result [Encrypted DynamoDB Item](./encrypt-item.md#encrypted-dynamodb-item)
         //# calculated above.
-        var put := Some(item.Put.value.(Item := encrypted.encryptedItem));
+        var put := Some(item.Put.value.(Item := encrypted.encryptedItem + beaconAttrs));
         var newItem := item.(Put := put);
         ghost var oldResult := result;
         result := result + [newItem];
